lean4.lean
@@ -1,0 +1,9 @@
+
+def main : IO Unit :=
+  IO.println "Hello, world!"
+
+theorem test1 {α} (a b : α) (as bs : List α) (h : a::as = b::bs) : a = b :=
+by {
+  injection h;
+  assumption;
+}
